(wip) open exhaustive

Core/Global.lean
@@ -50,7 +50,7 @@ abbrev GlobalEnv := List Global
 --   reprPrec a p := GlobalEnv.repr p a
 
 inductive Entry : Type where
-| data : String -> Kind -> Vec (String × SpineTy) n -> Entry
+| data : {n : Nat} -> String -> Kind -> Vec (String × SpineTy) n -> Entry
 | ctor : String -> Nat -> SpineTy -> Entry
 | odata : String -> Kind -> Entry
 | openm : String -> SpineTy -> Entry
@@ -183,7 +183,7 @@ def lookup_ctor_names (G : GlobalEnv) (T : Ty) : Option ((n : Nat) × Vec String
 @[simp]
 def pattern_match : Vec Constructor m -> Pattern m -> Bool
 | .nil, .nil => true
-| .cons ⟨q, m, As, n, _, k, _⟩ xs, .cons ⟨q', m', As', n', k'⟩ zs =>
+| .cons ⟨q, m, _, n, _, k, _⟩ xs, .cons ⟨q', m', _, n', k'⟩ zs =>
   pattern_match xs zs && q == q' && m == m' && n == n' && k == k' -- && As.beq As'
 | _, _ => false
 
@@ -212,160 +212,8 @@ def lookup_defn (G : List Global) (x : String) : Option (Ty × Term) := do
   | _ => none
 
 def lookup_kind G x := lookup x G |> Option.map Entry.kind |> Option.join
--- def lookup_type G x := lookup x G |> Option.map Entry.type |> Option.get!
--- def lookup_spctor_type G x := lookup x G |> Option.map Entry.spctor_type |> Option.get!
--- def is_ctor G x := lookup x G |> Option.map Entry.is_ctor |> Option.get!
 def is_data c G x := lookup x G |> Option.map (Entry.is_data c) |> Option.getD (dflt := false)
--- def is_instty G x := lookup x G |> Option.map Entry.is_instty |> Option.get!
--- def is_opent G x := lookup x G |> Option.map Entry.is_opent |> Option.get!
--- def is_openm G x := lookup x G |> Option.map Entry.is_openm |> Option.get!
--- def is_defn G x := lookup x G |> Option.map Entry.is_defn |> Option.get!
 
 
--- def ctor_idx (G : List Global) (x : String) : Option Nat := do
---   let t <- lookup x G
---   match t with
---   | .ctor _ n _ => n
---   | _ => none
-
--- def ctor_ty (G : List Global) (x : String) : Option Ty := do
---   let t <- lookup_type G x
---   if is_ctor G x then return t else none
-
--- def ctor_count (G : List Global) (x : String) : Option Nat := do
---   let t <- lookup x G
---   match t with
---   | .data _ _ ctors => Vec.length ctors
---   | _ => .none
-
-
--- theorem lookup_type_reconstruct :
---   lookup x G = some e ->
---   e.type = some T ->
---   lookup_type G x = some T
--- := by
---   intro j1 j2
---   simp [lookup_type]; rw [j1]; simp
---   exact j2
-
--- theorem lookup_entry_openm_exists :
---   is_openm G x -> ∃ y T, lookup x G = .some (Entry.openm y T) := by
--- intro h
--- simp [is_openm] at h
--- generalize edef : lookup x G = e at *
--- cases e <;> simp at h
--- case _ e =>
--- cases e <;> simp [Entry.is_openm] at h
--- case _ x T => exists x; exists T
-
--- theorem lookup_entry_defn_exists :
---   is_defn G x -> ∃ y T t, lookup x G = .some (Entry.defn y T t) := by
--- intro h
--- simp [is_defn] at h
--- generalize edef : lookup x G = e at *
--- cases e <;> simp at h
--- case _ e =>
--- cases e <;> simp [Entry.is_defn] at h
--- case _ y T t => exists y; exists T; exists t
-
--- theorem lookup_defn_is_defn_sound :
---   lookup_defn G x = .some t -> is_defn G x := by
--- intro h; rw[is_defn]; rw[lookup_defn] at h; simp [Option.bind] at h
--- generalize zdef : lookup x G = z at *
--- cases z <;> simp at *
--- case _ z =>
--- cases z <;> simp [Entry.is_defn] at *
-
--- theorem lookup_defn_some :
---   lookup_defn G x = .some t -> ∃ y T t, lookup x G = .some (Entry.defn y T t) := by
--- intro h1
--- replace h1 := lookup_defn_is_defn_sound h1
--- apply lookup_entry_defn_exists h1
-
--- theorem is_stable_implies_not_is_openm : is_stable G x -> ¬ is_openm G x := by
---   intro h1 h2
---   simp [is_stable] at h1;
---   cases h1
---   all_goals
---     case _ h1 =>
---       have lem := lookup_entry_openm_exists h2
---       rcases lem with ⟨_, _, lem⟩
---       simp [is_ctor, is_instty] at h1; rw[lem] at h1
---       simp at h1; simp [Entry.is_ctor, Entry.is_instty] at h1
--- grind_pattern is_stable_implies_not_is_openm => is_stable G x, is_openm G x
-
--- theorem is_stable_implies_not_is_defn : is_stable G x -> ¬ is_defn G x := by
---   intro h1 h2
---   simp [is_stable] at h1;
---   cases h1
---   all_goals
---     case _ h1 =>
---       have lem := lookup_entry_defn_exists h2
---       rcases lem with ⟨_, _, _, lem⟩
---       simp [is_ctor, is_instty] at h1; rw[lem] at h1
---       simp at h1; simp [Entry.is_ctor, Entry.is_instty] at h1
--- grind_pattern is_stable_implies_not_is_defn => is_stable G x, is_defn G x
-
--- theorem is_stable_implies_lookup_defn_none : is_stable G x -> lookup_defn G x = none := by
---   intro h
---   have lem := is_stable_implies_not_is_defn h
---   unfold is_defn at lem; unfold lookup_defn; simp
---   intro a h2; rw [h2] at lem; simp at lem
---   cases a <;> simp
---   simp [Entry.is_defn] at lem
--- grind_pattern is_stable_implies_lookup_defn_none => is_stable G x
-
--- theorem is_openm_implies_lookup_defn_none : is_openm G x -> lookup_defn G x = none := by
---   sorry
--- grind_pattern is_openm_implies_lookup_defn_none => is_openm G x
-
--- theorem not_stable_implies_openm_or_defn :
---   is_stable G x = false ->
---   (lookup_type G x).isSome ->
---   is_defn G x ∨ is_openm G x
--- := by
---   intro h1 h2
---   unfold is_stable at h1
---   unfold is_ctor at h1
---   unfold is_instty at h1
---   unfold lookup_type at h2
---   unfold is_defn; unfold is_openm
---   generalize zdef : lookup x G = z at *
---   cases z; simp [Option.isSome] at h2; case _ z =>
---   cases z <;> simp [Entry.type, Entry.is_ctor, Entry.is_instty] at *
---   all_goals simp [Entry.is_defn, Entry.is_openm]
-
--- theorem Global.lookup_unique :
---   lookup x G = t ->
---   lookup x G = t' ->
---   t = t'
--- := by
---   intro h1 h2
---   all_goals (rw[h1] at h2; exact h2)
-
--- theorem Global.lookup_type_unique :
---   lookup_type x G = some t ->
---   lookup_type x G = some t' ->
---   t = t' := by
--- intro h1 h2
--- all_goals (rw[h1] at h2; injection h2)
-
--- theorem Global.get_defn :
---   is_defn G x ->
---   ∃ T t, lookup x G = some (.defn x T t)
--- := by
---   intro h
---   unfold is_defn at h
---   generalize zdef : lookup x G = z at *
---   cases z; simp at h; case _ z =>
---   cases z <;> simp [Entry.is_defn] at h
---   simp
---   sorry
-
--- theorem Global.get_openm :
---   is_openm G x ->
---   ∃ T, lookup x G = some (.openm x T)
--- := by
---   sorry
 
 end Core
